Excalead/domin8/model/instructions/deposit_bet.v
@@ -1,4 +1,4 @@
-Require Import Excalead.Excalead.
+From Excalead Require Import Excalead Tactics Vector.
 
 From Excalead.domin8.model Require Import state.mod errors constants.
 
@@ -116,3 +116,41 @@ Definition deposit_bet
     (* msg!("Total pot: {} lamports", game_round.initial_pot); *)
 
   Result.Ok game_round.
+
+Lemma deposit_bet_is_valid (ctx : Context.t DepositBet.t) (amount : u64)
+    (H_param1 : GameRound.Valid.t ctx.(Context.accounts).(DepositBet.game_round)) :
+  match deposit_bet ctx amount with
+  | Result.Ok (result1) => GameRound.Valid.t result1
+  | Result.Err _ => True
+  end.
+Proof.
+  unfold deposit_bet.
+  step; step; step; step; step;
+    match goal with | H: SystemProgram.transfer _ _ = _ |- _ => clear H end.
+  match goal with
+  | |- context [ GameRound.find_player_mut ?game_round _ ] =>
+    remember game_round as game_round' eqn:HeqGameRound;
+    assert (Hgame_round'_length:
+        Z.of_nat (Datatypes.length game_round'.(GameRound.players)) < MAX_PLAYERS)
+      by (subst; step; simpl; lia);
+    clear HeqGameRound
+  end.
+
+  unfold GameRound.find_player_mut.
+  match goal with
+  | |- context [Vector.zipper_find ?pred' ?vec' ] =>
+    set (pred:=pred'); clearbody pred;
+    destruct (Vector.zipper_spec pred vec')
+  end.
+  + (* If GameRound.find_player_mut didn't find the player *)
+    rewrite Hresult.
+    constructor.
+    simpl; lia.
+  + (* If GameRound.find_player_mut did find the player *)
+    rewrite Hresult.
+    constructor.
+    simpl.
+    rewrite unzipper_length with (x := x), <- Hunzip.
+    lia.
+Qed.
+
